coq/theories/ITree/Monad.v
@@ -20,8 +20,6 @@ Section monad.
          | VisF e k => VisF e (fun r => _fmap _ (k r))
          end).
 
-  Print respectful.
-
   #[global] Instance fmap_eq {X RX Y RY} {f : X ⇒ᵢ Y}
     {_ : forall i, Proper (@RX i ==> @RY i) (f i)}
     {i} : Proper (it_eq RX (i:=i) ==> it_eq RY (i:=i)) (fmap f i).
@@ -41,51 +39,86 @@ Section monad.
          | VisF e k => VisF e (fun r => _subst _ (k r))
           end).
 
-  #[global] Instance subst_eq {X Y}
-    : Proper (dpointwise_relation (fun i => pointwise_relation (X i) (it_eq (i:=i)))
-                ==> dpointwise_relation (fun i => it_eq (i:=i) ==> (it_eq (i:=i))))
+  #[global] Instance subst_eq {X Y} {RX : relᵢ X X} {RY : relᵢ Y Y}
+    : Proper (dpointwise_relation (fun i => RX i ==> it_eq RY (i:=i))
+              ==> dpointwise_relation (fun i => it_eq RX (i:=i) ==> it_eq RY (i:=i)))
         (@subst X Y).
   Proof.
     unfold Proper, respectful, dpointwise_relation, pointwise_relation, it_eq.
     intros f g h1; coinduction R CIH; intros i x y h2.
-    apply (gfp_fp (it_eq_map E X)) in h2.
+    apply (gfp_fp (it_eq_map E RX)) in h2.
     cbn in *; cbv [observe] in h2; dependent destruction h2; simpl_depind; eauto.
-    pose (h3 := h1 i r).
-    apply (gfp_fp (it_eq_map E Y)) in h3.
+    pose (h3 := h1 i _ _ r_rel).
+    apply (gfp_fp (it_eq_map E RY)) in h3.
     cbn in h3; cbv [observe] in h3.
-    dependent destruction h3; simpl_depind; econstructor.
-    2: intro r0.
-    all: now apply (gfp_t (it_eq_map E Y)).
+    dependent destruction h3; simpl_depind; econstructor; eauto.
+    2: intro.
+    all: now apply (gfp_t (it_eq_map E RY)).
   Qed.
+  
+  #[global] Instance subst_eat {X Y} (f : X ⇒ᵢ itree E Y) {i}
+   : Proper (it_eat' i ==> it_eat' i) (subst f i).
+  Proof.
+    intros ? ? H; unfold it_eat' in *; cbn.
+    dependent induction H; simpl_depind; econstructor; cbn; eauto.
+  Qed.    
 
   Definition bind {X Y i} x f := @subst X Y f i x.
 
-  Variant bindR {X Y} (R : relᵢ (itree E X) (itree E X)) (S : relᵢ (itree E Y) (itree E Y))
+  Variant bindR {X Y} (RX : relᵢ X X) (R : relᵢ (itree E X) (itree E X))
+                (S : relᵢ (itree E Y) (itree E Y))
           : relᵢ (itree E Y) (itree E Y) :=
     | BindR {i t1 t2 k1 k2}
         (u : R i t1 t2)
-        (v : forall i x, S i (k1 i x) (k2 i x))
-      : bindR R S i (bind t1 k1) (bind t2 k2).
-  Arguments BindR {X Y R S i t1 t2 k1 k2}.    
+        (v : forall i x1 x2, RX i x1 x2 -> S i (k1 i x1) (k2 i x2))
+      : bindR RX R S i (bind t1 k1) (bind t2 k2).
+  Arguments BindR {X Y RX R S i t1 t2 k1 k2}.    
   Hint Constructors bindR : core.
 
-  Program Definition bindR_map {X Y} : mon (relᵢ (itree E Y) (itree E Y)) :=
-    {| body S := bindR (@it_eq _ E X) S ;
-       Hbody _ _ H _ _ _ '(BindR u v) := BindR u (fun i x => H _ _ _ (v i x)) |}.
+  Program Definition bindR_eq_map {X Y} (RX : relᵢ X X) : mon (relᵢ (itree E Y) (itree E Y)) :=
+    {| body S := bindR RX (@it_eq _ E _ RX) S ;
+       Hbody _ _ H _ _ _ '(BindR u v) := BindR u (fun i _ _ r => H _ _ _ (v i _ _ r)) |}.
 
-  Lemma it_eq_up2bind_t {X Y} : @bindR_map X Y <= it_eq_t E Y.
+  Lemma it_eq_up2bind_t {X Y} RX RY : @bindR_eq_map X Y RX <= it_eq_t E RY.
   Proof.
     apply Coinduction; intros R i x y [ ? ? ? ? ? u v].
-    unfold it_eq in u; apply (gfp_fp (it_eq_map E X)) in u.
+    unfold it_eq in u; apply (gfp_fp (it_eq_map E RX)) in u.
     cbn in *; cbv [observe] in u.
     dependent destruction u; simpl_depind.
-    - refine (it_eqF_mon _ _ (id_T _ _ R) _ _ _ (v i0 r)).
-    - econstructor; apply (fTf_Tf (it_eq_map E Y)).
-      refine (BindR t_rel (fun i r => b_T (it_eq_map E Y) _ _ _ _ _ (v i r))).
-    - econstructor; intros r; apply (fTf_Tf (it_eq_map E Y)).
-      refine (BindR (k_rel r) (fun i r => b_T (it_eq_map E Y) _ _ _ _ _ (v i r))).
+    - refine (it_eqF_mon _ _ (id_T _ _ R) _ _ _ (v i0 _ _ r_rel)).
+    - econstructor; apply (fTf_Tf (it_eq_map E RY)).
+      refine (BindR t_rel (fun i _ _ r => b_T (it_eq_map E RY) _ _ _ _ _ (v i _ _ r))).
+    - econstructor; intros r; apply (fTf_Tf (it_eq_map E RY)).
+      refine (BindR (k_rel r) (fun i _ _ r => b_T (it_eq_map E RY) _ _ _ _ _ (v i _ _ r))).
   Qed.
 
+  Program Definition bindR_w_map {X Y} (RX : relᵢ X X) : mon (relᵢ (itree E Y) (itree E Y)) :=
+    {| body S := bindR RX (@it_wbisim _ E _ RX) S ;
+       Hbody _ _ H _ _ _ '(BindR u v) := BindR u (fun i _ _ r => H _ _ _ (v i _ _ r)) |}.
+
+  Lemma it_wbisim_up2bind_t {X Y} RX RY : @bindR_w_map X Y RX <= it_wbisim_t E RY.
+  Proof.
+    apply Coinduction; intros R i x y [ ? ? ? ? ? u v].
+    unfold it_wbisim in u; apply (gfp_fp (it_wbisim_map E RX)) in u.
+    cbn in *; cbv [observe] in u.
+    destruct u as [? ? r1 r2 rr]; dependent destruction rr.
+    - destruct (v _ _ _ r_rel) as [ ? ? s1 s2 ss]; econstructor.
+      etransitivity; [ exact (subst_eat _ _ (Ret' _) r1) | exact s1 ].
+      etransitivity; [ exact (subst_eat _ _ (Ret' _) r2) | exact s2 ].
+      now apply (it_eqF_mon _ _ (id_T _ _ R)).
+   - econstructor.
+     exact (subst_eat _ _ (Tau' _) r1).
+     exact (subst_eat _ _ (Tau' _) r2).
+     cbn; econstructor.
+     apply (fTf_Tf (it_wbisim_map E RY)).
+     econstructor; [ apply t_rel | intros; now apply (b_T (it_wbisim_map E RY)), v ].
+   - econstructor.
+     exact (subst_eat _ _ (Vis' _ _) r1).
+     exact (subst_eat _ _ (Vis' _ _) r2).
+     cbn; econstructor; intro r.
+     apply (fTf_Tf (it_wbisim_map E RY)).
+     econstructor; [ apply k_rel | intros; now apply (b_T (it_wbisim_map E RY)), v ].
+ Qed.
 
   Definition kcomp {X Y Z} (f : X ⇒ᵢ itree E Y) (g : Y ⇒ᵢ itree E Z) : X ⇒ᵢ itree E Z :=
     fun i x => bind (f i x) g.
@@ -96,63 +129,102 @@ Section monad.
                                 | inl x => TauF (_iter _ x)
                                 | inr y => RetF y end)) .
 
-  #[global] Instance iter_eq {X Y}
-    : Proper (dpointwise_relation (fun i => pointwise_relation (X i) (it_eq (i:=i)))
-                ==> dpointwise_relation (fun i => pointwise_relation (X i) (it_eq (i:=i))))
+  #[global] Instance iter_eq {X Y} {RX : relᵢ X X} {RY : relᵢ Y Y}
+    : Proper (dpointwise_relation (fun i => RX i ==> it_eq (sumᵣ RX RY) (i:=i))
+              ==> dpointwise_relation (fun i => RX i ==> it_eq RY (i:=i)))
              (@iter X Y).
   Proof.
     unfold Proper, respectful, dpointwise_relation, pointwise_relation, it_eq.
-    intros f g h1; coinduction R CIH; intros i x.
-    pose (h3 := h1 i x).
-    apply (gfp_fp (it_eq_map E _)) in h3.
+    intros f g h1; coinduction R CIH; intros i x y r.
+    pose (h3 := h1 i x y r).
+    apply (gfp_fp (it_eq_map E (sumᵣ RX RY))) in h3.
     cbn in *; cbv [observe] in h3.
     dependent destruction h3; simpl_depind.
-    - destruct r; eauto.
+    - destruct r_rel; eauto.
     - econstructor.
       apply (tt_t (it_eq_map E _)); cbn.
-      apply (@it_eq_up2bind_t (X +ᵢ Y)); econstructor; eauto.
-      intros ? []; apply (tt_t (it_eq_map E Y)), (b_t (it_eq_map E Y)); cbn; eauto.
-    - econstructor; intro r.
+      apply (it_eq_up2bind_t (sumᵣ RX RY) RY); econstructor; eauto.
+      intros ? ? ? []; apply (tt_t (it_eq_map E RY)), (b_t (it_eq_map E RY)); cbn; eauto.
+    - econstructor; intro.
       apply (tt_t (it_eq_map E _)); cbn.
-      apply (@it_eq_up2bind_t (X +ᵢ Y)); econstructor; eauto.
+      apply (it_eq_up2bind_t (sumᵣ RX RY) RY); econstructor; eauto.
       apply k_rel.
-      intros ? []; apply (bt_t (it_eq_map E Y)); cbn; eauto.
+      intros ? ? ? []; apply (bt_t (it_eq_map E RY)); cbn; eauto.
   Qed.
 
-  Lemma iter_unfold {X Y} (f : X ⇒ᵢ itree E (X +ᵢ Y)) {i x}
-    : it_eq
+  #[global] Instance iter_weq {X Y} {RX : relᵢ X X} {RY : relᵢ Y Y}
+    : Proper (dpointwise_relation (fun i => RX i ==> it_wbisim (sumᵣ RX RY) (i:=i))
+              ==> dpointwise_relation (fun i => RX i ==> it_wbisim RY (i:=i)))
+             (@iter X Y).
+  Proof.
+    unfold Proper, respectful, dpointwise_relation, pointwise_relation, it_wbisim.
+    intros f g h1; coinduction R CIH; intros i x y r.
+    pose (h3 := h1 i x y r).
+    apply (gfp_fp (it_wbisim_map E (sumᵣ RX RY))) in h3.
+    cbn in *; cbv [observe] in h3.
+    destruct h3 as [ ? ? r1 r2 rr ]; dependent destruction rr.
+    - destruct r_rel.
+      * pose (H3 := h1 _ _ _ H).
+        apply (gfp_fp (it_wbisim_map E _)) in H3.
+        destruct H3 as [ ? ? s1 s2 ss ].
+        econstructor.
+        exact (subst_eat _ _ (Ret' _) r1).
+        exact (subst_eat _ _ (Ret' _) r2).
+        econstructor.
+        now apply CIH.
+      * econstructor.
+        exact (subst_eat _ _ (Ret' _) r1).
+        exact (subst_eat _ _ (Ret' _) r2).
+        now econstructor.
+    - econstructor.
+      exact (subst_eat _ _ (Tau' _) r1).
+      exact (subst_eat _ _ (Tau' _) r2).
+      cbn; econstructor.
+      apply (tt_t (it_wbisim_map E _)); cbn.
+      apply (it_wbisim_up2bind_t (sumᵣ RX RY) RY); econstructor; eauto.
+      intros ? ? ? []; apply (tt_t (it_wbisim_map E RY)), (b_t (it_wbisim_map E RY)); cbn; eauto.
+    - econstructor.
+      exact (subst_eat _ _ (Vis' _ _) r1).
+      exact (subst_eat _ _ (Vis' _ _) r2).
+      cbn; econstructor; intro.
+      apply (tt_t (it_wbisim_map E _)); cbn.
+      apply (it_wbisim_up2bind_t (sumᵣ RX RY) RY); econstructor; [ apply k_rel | ].
+      intros ? ? ? []; apply (tt_t (it_wbisim_map E RY)), (b_t (it_wbisim_map E RY)); cbn; eauto.
+  Qed.
+
+  Lemma iter_unfold {X Y RY} {_ : Reflexiveᵢ RY} (f : X ⇒ᵢ itree E (X +ᵢ Y)) {i x}
+    : it_eq RY
         (iter f i x)
         (bind (f i x) (fun _ r => go (match r with
                                    | inl x => TauF (iter f _ x)
                                    | inr y => RetF y end))).
   Proof.
-    apply (gfp_fp (it_eq_map E Y)).
+    apply (gfp_fp (it_eq_map E RY)).
     cbn; destruct (_observe (f i x)); auto.
-    destruct r; auto.
+    destruct r; eauto.
   Qed.
   
-  Lemma iter_lem {X Y} (f : X ⇒ᵢ itree E (X +ᵢ Y)) (g : X ⇒ᵢ itree E Y)
-                 (H : forall i x, it_eq (g i x) (bind (f i x) (fun _ r => go (match r with
+  Lemma iter_lem {X Y RY} {_ : Equivalenceᵢ RY} (f : X ⇒ᵢ itree E (X +ᵢ Y)) (g : X ⇒ᵢ itree E Y)
+                 (H : forall i x, it_eq RY (g i x) (bind (f i x) (fun _ r => go (match r with
                                                   | inl x => TauF (g _ x)
                                                   | inr y => RetF y end))))
-                 : forall i x, it_eq (g i x) (iter f i x).
+                 : forall i x, it_eq RY (g i x) (iter f i x).
   Proof.
     unfold it_eq; coinduction R CIH; intros i x.
-    apply (bt_tbt (it_eq_map E Y)).
+    apply (bt_tbt (it_eq_map E RY)).
     etransitivity.
-    now unshelve eapply (Hbody (it_eq_t E Y) _ _ _ _ _ _ (H i x)).
-    etransitivity.
-    all: cycle 1.
-    symmetry.
-    now unshelve eapply (Hbody (it_eq_t E Y) _ _ _ _ _ _ (iter_unfold f)).
-    eapply (@it_eq_up2bind_t (X +ᵢ Y) Y).
+    now unshelve eapply (Hbody (it_eq_t E RY) _ _ _ _ _ _ (H i x)).
+    etransitivity; cycle 1.
+    symmetry; now unshelve eapply (Hbody (it_eq_t E RY) _ _ _ _ _ _ (iter_unfold f)).
+    eapply (it_eq_up2bind_t (eqᵢ (X +ᵢ Y)) RY).
     econstructor. reflexivity.
-    intros ? []; econstructor.
+    intros ? ? [] ->; econstructor.
     now apply CIH.
+    reflexivity.
   Qed.
 
-  Lemma bind_bind_com {X Y Z} {f : X ⇒ᵢ itree E Y} {g : Y ⇒ᵢ itree E Z} {i} {x : itree E X i}
-    : it_eq (bind (bind x f) g) (bind x (kcomp f g)).
+  Lemma bind_bind_com {X Y Z RZ} {_ : Reflexiveᵢ RZ} {f : X ⇒ᵢ itree E Y} {g : Y ⇒ᵢ itree E Z} {i} {x : itree E X i}
+    : it_eq RZ (bind (bind x f) g) (bind x (kcomp f g)).
   Proof.
     revert i x; unfold it_eq; coinduction R CIH; intros i x.
     cbn; destruct (x.(_observe)); eauto.
@@ -160,16 +232,16 @@ Section monad.
     destruct ((g i r0).(_observe)); eauto.
   Qed.
 
-  Lemma fmap_bind_com {X Y Z} {f : X ⇒ᵢ Y} {g : Y ⇒ᵢ itree E Z} {i} {x : itree E X i}
-    : it_eq (bind (fmap f _ x) g) (bind x (fun i x => g i (f i x))).
+  Lemma fmap_bind_com {X Y Z RZ} {_ : Reflexiveᵢ RZ} {f : X ⇒ᵢ Y} {g : Y ⇒ᵢ itree E Z} {i} {x : itree E X i}
+    : it_eq RZ (bind (fmap f _ x) g) (bind x (fun i x => g i (f i x))).
   Proof.
     revert i x; unfold it_eq; coinduction R CIH; intros i x.
     cbn; destruct (x.(_observe)); eauto.
     destruct ((g i (f i r)).(_observe)); eauto.
   Qed.
 
-  Lemma bind_fmap_com {X Y Z} {f : X ⇒ᵢ itree E Y} {g : Y ⇒ᵢ Z} {i} {x : itree E X i}
-    : it_eq (fmap g _ (bind x f)) (bind x (fun i x => fmap g i (f i x))).
+  Lemma bind_fmap_com {X Y Z RZ} {_ : Reflexiveᵢ RZ} {f : X ⇒ᵢ itree E Y} {g : Y ⇒ᵢ Z} {i} {x : itree E X i}
+    : it_eq RZ (fmap g _ (bind x f)) (bind x (fun i x => fmap g i (f i x))).
   Proof.
     revert i x; unfold it_eq; coinduction R CIH; intros i x.
     cbn; destruct (x.(_observe)); eauto.
